theories/Relational/GenericRulesComplex.v
@@ -43,94 +43,7 @@ Section RelationalProgramLogicFromRelativeMonad.
   Import SPropNotations.
   Import RelNotations.
 
-  Notation " Γ ⊫ c1 ≈ c2 [{ w1 , w2 , w }]" :=
-    ((forall γ1 : πl Γ, (θ1 _)∙1 (c1 γ1) ≤ Spr1 w1 γ1) s/\
-    (forall γ2 : πr Γ, (θ2 _)∙1 (c2 γ2) ≤ Spr1 w2 γ2) s/\
-    (forall γ : ⟬Γ⟭, θW∙1 ⟨c1 (πl γ), c2 (πr γ)⟩ ≤ Spr1 w (dfst γ)))
-      (at level 85).
 
-  Notation "⋅⊫ c1 ≈ c2 [{ w1 , w2 , w }]" :=
-    (Hi unit ⊫ (fun=> c1) ≈ (fun=> c2) [{ @OrdCat_cst (discr unit) _ w1,
-                                    @OrdCat_cst (discr unit) _ w2,
-                                    @OrdCat_cst (discr (unit × unit)) _ w}]).
-
-  Check (fun A B (c1 : M1 A) (c2: M2 B) (w1:dfst (W1 A)) (w2:dfst (W2 B)) (w3:dfst (W0 ⟨A,B⟩)) => ⋅⊫ c1 ≈ c2 [{ w1, w2, w3 }] ).
-
-
-  Lemma equal_f {A B} (x:A) (f g : forall x:A, B x) : f = g -> f x = g x.
-  Proof. move=> ? ; f_equal=> //. Qed.
-
-  Lemma ordCat_helper {A B} (f g : OrdCat⦅A;B⦆) : f ⪷ g -> forall (x y:dfst A), x ≤ y -> f∙1 x ≤ g∙1 y.
-  Proof.
-    move=> Hfg x y Hxy; estransitivity.
-    apply: (f∙2); exact: Hxy.
-    apply: Hfg.
-  Qed.
-
-  (* And we prove the rule for binding computations *)
-
-  Lemma full_seq_rule {A1 A2 B1 B2}
-        {m1 : M1 A1} {m2 : M2 A2} {wm1 wm2 wm}
-        {f1 : A1 -> M1 B1} {f2 : A2 -> M2 B2}
-        {wf1 : OrdCat⦅discr A1; W1 B1⦆} {wf2:OrdCat⦅discr A2;W2 B2⦆}
-        {wf : OrdCat⦅Jprod ⟨A1,A2⟩ ; W0 ⟨B1, B2⟩⦆} :
-    ⋅⊫ m1 ≈ m2 [{ wm1, wm2, wm }] ->
-    (⦑A1,A2|fun=>fun=>unit|TyRel⦒ ⊫ f1 ≈ f2 [{ wf1, wf2,  wf }]) ->
-    ⋅⊫ bind m1 f1 ≈ bind m2 f2 [{ wm1 ≫= wf1,
-                                  wm2 ≫= wf2,
-                                  (actW wf1 wf2 wf)∙1 wm }].
-  Proof.
-    intros [[Hm1 Hm2] Hm] [[Hf1 Hf2] Hf].
-    split;[split|]=> ?.
-    - move: (rmm_law2 _ _ _ _ θ1 _ _ f1)=> /(f_equal (fun f=> f∙1 m1)) /= ->.
-      apply: ordCat_helper; last by apply: Hm1.
-      apply: (ord_relmon_bind_proper W1); apply: Hf1.
-    - move: (rmm_law2 _ _ _ _ θ2 _ _ f2)=> /(f_equal (fun f=> f∙1 m2)) /= ->.
-      apply: ordCat_helper; last by apply: Hm2.
-      apply: (ord_relmon_bind_proper W2); apply: Hf2.
-    - move: (reoc_law2 _ _ _ _ _ θrc (to_prod f1 f2))
-        => /(f_equal (fun f=> f∙1 ⟨m1,m2⟩)) /= ->; estransitivity.
-      apply: rsmc_act_proper;
-        [apply: Hf1| apply: Hf2| move=> [? ?] /=; eapply (Hf ⦑ _ , _ | tt⦒)].
-      eapply ((actW _ _ _)∙2)=> //; apply (Hm ⦑tt,tt|I⦒).
-  Qed.
-
-    (* move: (rmm_law2 _ _ M12 (W' W) θ _ _ (to_prod f1 f2))=> /= [[H1 H2] H12]. *)
-    (* intuition. *)
-    (* move: (f_equal (fun h => h m1) H1)=> /= ->. *)
-    (* apply omon_bind=> //; apply (Hm1 tt). *)
-    (* move: (f_equal (fun h => h m2) H2)=> /= ->. *)
-    (* apply omon_bind=> //; apply (Hm2 tt). *)
-    (* move: (f_equal (fun h => h ⟨m1, m2⟩) H12) => /= -> //=. *)
-    (* estransitivity. *)
-    (* simpl in Hf1. *)
-    (* apply: rsmc_act_proper. *)
-    (* move=> ? ; apply Hf1. *)
-    (* move=> ? ; apply Hf2. *)
-    (* move=> [? ?] /=; eapply (Hf ⦑ _ , _ | tt⦒). *)
-    (* eapply (Spr2 (actW _ _ _))=> //. *)
-    (* apply (Hm ⦑tt,tt|I⦒). *)
-
-  (* Program Definition bindWrelStrong *)
-  (*       {Γ A1 A2 B1 B2} *)
-  (*       (wm1 : OrdCat⦅discr (πl Γ); W1 A1⦆) *)
-  (*       (wm2 : OrdCat⦅discr (πr Γ); W2 A2⦆) *)
-  (*       (wmrel : OrdCat⦅discr ⟬Γ⟭; Wrel ⟨A1, A2⟩⦆) *)
-  (*       (wf1 : OrdCat⦅discr (πl Γ × A1); W1 B1⦆) *)
-  (*       (wf2 : OrdCat⦅discr (πr Γ × A2); W2 B2⦆) *)
-  (*       (wfrel : OrdCat⦅discr ⟬extends Γ A1 A2⟭; Wrel ⟨B1, B2⟩⦆) *)
-  (*   : OrdCat⦅discr ⟬Γ⟭; Wrel ⟨B1, B2⟩⦆ := *)
-  (*   ⦑fun γ => (actW (wf1 ∙ ofmap discr (fun a1 => ⟨πl γ, a1⟩)) *)
-  (*                (wf2 ∙ ofmap discr (fun a2 => ⟨πr γ, a2⟩)) *)
-  (*                (wfrel ∙ ofmap discr (fun a12 => extend_point γ (nfst a12) (nsnd a12))) ∙ wmrel)∙1 γ ⦒. *)
-  (* Next Obligation. *)
-  (*   cbv=> ? ?; induction 1 ; apply: rsmc_act_proper; sreflexivity. *)
-  (* Qed. *)
-
-  Notation " X --> Y " := (X -> dfst Y) (at level 99).
-
-  Program Definition to_discr {X Y} (f : X --> Y) : OrdCat⦅discr X; Y⦆ := ⦑f⦒.
-  Next Obligation. move=> ? ?; induction 1; sreflexivity. Qed.
 
   Definition bindWrelStrong {Γ A1 A2 B1 B2}
           (wm1 : πl Γ --> W1 A1) (wm2 : πr Γ --> W2 A2)
@@ -153,11 +66,6 @@ Section RelationalProgramLogicFromRelativeMonad.
   Notation prog2 c := (nfst \o πr c).
   Notation spec2 c := (nsnd \o πr c).
   Notation specrel c := (πw c).
-  (* Definition prog1 {Γ A1 A2} (c : progSpec Γ A1 A2) := nfst \o πl c. *)
-  (* Definition spec1 {Γ A1 A2} (c : progSpec Γ A1 A2) := nsnd \o πl c. *)
-  (* Definition prog2 {Γ A1 A2} (c : progSpec Γ A1 A2) := nfst \o πr c. *)
-  (* Definition spec2 {Γ A1 A2} (c : progSpec Γ A1 A2) := nsnd \o πr c. *)
-  (* Definition specrel {Γ A1 A2} (c : progSpec Γ A1 A2) := πw c. *)
 
   Definition mk_progSpec
              (Γ : Rel) A1 A2
@@ -186,7 +94,8 @@ Section RelationalProgramLogicFromRelativeMonad.
   Definition valid Γ {A1 A2} (c : progSpec Γ A1 A2) := ⟬dArr (validity c)⟭.
 
   Notation " Γ ⊫ c1 ≈ c2 [{ w1 , w2 , w }] " :=
-    (valid Γ (mk_progSpec Γ _ _ c1 w1 c2 w2 w)).
+    (valid Γ (mk_progSpec Γ _ _ c1 w1 c2 w2 w))
+      (at level 85).
 
 
   Definition retWrel {A1 A2} : A1 -> A2 --> Wrel ⟨A1,A2⟩ :=
@@ -389,12 +298,6 @@ Section RelationalProgramLogicFromRelativeMonad.
   Notation subst_inr := (prodl inr).
   Notation rel_subst_inr := (rel_prodl inr).
 
-  (* Definition subst_inl {X Y} := prodl (@inl X Y). *)
-  (* Definition rel_subst_inl := rel_prodl inl. *)
-  (* Definition subst_inr := prodl inr. *)
-  (* Definition rel_subst_inr := rel_prodl inr. *)
-
-
   Lemma ValidSumElim Γ X Y A1 A2 (m1: _ -> M1 A1) wm1 (m2: _ -> M2 A2) wm2 wmrel:
     (Γ,∙ X) ⊫ m1 \o subst_inl ≈ m2 \o subst_inl
      [{wm1 \o subst_inl, wm2 \o subst_inl, wmrel \o rel_subst_inl}] ->
@@ -416,182 +319,5 @@ Section RelationalProgramLogicFromRelativeMonad.
       [apply: (HL ⟨_,_⟩ ⟨_,_⟩ ⟨_,erefl⟩)|
       apply: (HR ⟨_,_⟩ ⟨_,_⟩ ⟨_,erefl⟩)].
   Qed.
-
-  (* Definition valid {Γ A1 A2} (c : progSpec Γ A1 A2) : Rel := *)
-  (*   mkRel (Box (forall γ1 : πl Γ, (θ1 _)∙1 (prog1 c γ1) ≤  spec1 c γ1)) *)
-  (*         (Box (forall γ2 : πr Γ, (θ2 _)∙1 (prog2 c γ2) ≤ spec2 c γ2)) *)
-  (*         (fun _ _ => Box (forall γ : ⟬Γ⟭, θW∙1 ⟨prog1 c (πl γ), prog2 c (πr γ)⟩ ≤ specrel c (πl γ) (πr γ) (πw γ))). *)
-
-  (* Definition valid (Γ : Rel) A1 A2 *)
-  (*            (c1: πl Γ -> M1 A1) (w1: πl Γ --> W1 A1) *)
-  (*            (c2:πr Γ -> M2 A2) (w2:πr Γ --> W2 A2) *)
-  (*            (wrel: ⟬Γ⟭ --> Wrel ⟨A1, A2⟩) : SProp := *)
-  (*   ((forall γ1 : πl Γ, (θ1 _)∙1 (c1 γ1) ≤  w1 γ1) s/\ *)
-  (*   (forall γ2 : πr Γ, (θ2 _)∙1 (c2 γ2) ≤ w2 γ2) s/\ *)
-  (*   (forall γ : ⟬Γ⟭, θW∙1 ⟨c1 (πl γ), c2 (πr γ)⟩ ≤ wrel γ)). *)
-
-  (* Definition retWrel {A1 A2} : A1 -> A2 --> Wrel ⟨A1,A2⟩ := *)
-  (*   fun a1 a2 => (rsmc_return Wrel ⟨A1,A2⟩)∙1 ⟨a1, a2⟩. *)
-
-  (* Definition retW {W : unarySpecMonad} {A} : A --> W A := (ord_relmon_unit W A)∙1. *)
-
-  (* Lemma ValidRet Γ A1 A2 a1 a2: *)
-  (*   valid Γ A1 A2  (ret \o a1)  (retW \o a1) (ret \o a2) (retW \o a2) *)
-  (*         (fun γ => retWrel (a1 (πl γ)) (a2 (πr γ))). *)
-  (* Proof. *)
-  (*   split;[split|]=> γ. *)
-  (*   - move: (rmm_law1 _ _ _ _ θ1 A1) => /(f_equal (fun f=> f∙1 (a1 γ))) /= ->. *)
-  (*     sreflexivity. *)
-  (*   - move: (rmm_law1 _ _ _ _ θ2 A2) => /(f_equal (fun f=> f∙1 (a2 γ))) /= ->. *)
-  (*     sreflexivity. *)
-  (*   - move: (@reoc_law1 _ _ _ _ _ _ _ θrc ⟨A1,A2⟩) *)
-  (*     => /(f_equal (fun f=> f∙1 ⟨a1 (πl γ), a2 (πr γ)⟩)) /= ->. *)
-  (*     sreflexivity. *)
-  (* Qed. *)
-
-
-  (* Definition bindWStr {W : unarySpecMonad} {Γ A B} *)
-  (*            (wm: Γ --> W A) (wf : Γ × A --> W B) : Γ --> W B := *)
-  (*   fun γ => (ord_relmon_bind W (to_discr (fun a => wf⟨γ, a⟩)))∙1 (wm γ). *)
-
-  (* Lemma ValidBind *)
-  (*       Γ A1 A2 B1 B2 m1 wm1 m2 wm2 wmrel f1 wf1 f2 wf2 wfrel : *)
-  (*   valid Γ A1 A2 m1 wm1 m2 wm2 wmrel -> *)
-  (*   valid (extends Γ A1 A2) B1 B2 f1 wf1 f2 wf2 wfrel -> *)
-  (*   valid Γ B1 B2 *)
-  (*         (bindStr m1 f1) (bindWStr wm1 wf1) *)
-  (*         (bindStr m2 f2) (bindWStr wm2 wf2) *)
-  (*         (bindWrelStrong wm1 wm2 wmrel wf1 wf2 wfrel). *)
-  (* Proof. *)
-  (*   move=> [[Hm1 Hm2] Hm] [[Hf1 Hf2] Hf]. *)
-  (*   split; [split|]=> γ. *)
-  (*   - move: (rmm_law2 _ _ _ _ θ1 _ _ (fun a => f1 ⟨γ,a⟩)) *)
-  (*     => /(f_equal (fun f=> f∙1 (m1 γ))) /= ->. *)
-  (*     apply: ordCat_helper; last by apply: Hm1. *)
-  (*     apply: (ord_relmon_bind_proper W1)=> ? ; apply: Hf1. *)
-  (*   - move: (rmm_law2 _ _ _ _ θ2 _ _ (fun a=> f2 ⟨γ,a⟩)) *)
-  (*     => /(f_equal (fun f=> f∙1 (m2 γ))) /= ->. *)
-  (*     apply: ordCat_helper; last by apply: Hm2. *)
-  (*     apply: (ord_relmon_bind_proper W2)=> ?; apply: Hf2. *)
-  (*   - move: (reoc_law2 _ _ _ _ _ θrc (to_prod (fun a=> f1 ⟨πl γ,a⟩) (fun a=> f2 ⟨πr γ,a⟩))) => /=. *)
-  (*     move=> /(f_equal (fun f=> f∙1 ⟨m1 (πl γ),m2 (πr γ)⟩)) /= ->; estransitivity; *)
-  (*     last (eapply ((actW _ _ _)∙2)=> //; apply (Hm ⦑tt,tt|I⦒)). *)
-  (*     apply: rsmc_act_proper; *)
-  (*       [move=> ? ; apply: Hf1| move=> ?; apply: Hf2|]. *)
-  (*     move=> [? ?] /=; set γ' := extend_point _ _ _; apply: (Hf γ'). *)
-  (* Qed. *)
-
-  (* Notation "x ⩿ y" := (pointwise_srelation _ (@extract_ord _) x y) (at level 70). *)
-
-  (* Lemma ValidWeaken *)
-  (*            Γ A1 A2 m1 wm1 wm1' m2 wm2 wm2' wmrel wmrel': *)
-  (*   valid Γ A1 A2 m1 wm1 m2 wm2 wmrel -> *)
-  (*   wm1 ⩿ wm1' -> wm2 ⩿ wm2' -> wmrel ⩿ wmrel' -> *)
-  (*   valid Γ A1 A2 m1 wm1' m2 wm2' wmrel'. *)
-  (* Proof. *)
-  (*   move=> [[H1 H2] H] Hle1 Hle2 Hle; split; [split|] => ?; estransitivity. *)
-  (*   apply: H1. apply: Hle1. *)
-  (*   apply: H2. apply: Hle2. *)
-  (*   apply: H. apply: Hle. *)
-  (* Qed. *)
-
-  (* Lemma ValidSubst Γ Δ A1 A2 m1 wm1 m2 wm2 wmrel (σ: Δ R==> Γ) : *)
-  (*   valid Γ A1 A2 m1 wm1 m2 wm2 wmrel -> *)
-  (*   valid Δ A1 A2 *)
-  (*         (m1 \o πl σ) (wm1 \o πl σ) *)
-  (*         (m2 \o πr σ) (wm2 \o πr σ) *)
-  (*         (wmrel \o applyRel _ _ σ). *)
-  (* Proof. *)
-  (*   move=> [[H1 H2] H]; split; [split|]=> γ. *)
-  (*   apply: H1. *)
-  (*   apply: H2. *)
-  (*   set γ' := (σ @R γ); exact: (H γ'). *)
-  (* Qed. *)
-
-  (* Definition subst_true {Γ} : Γ -> Γ × bool := fun γ => ⟨γ, true⟩. *)
-  (* Definition rel_subst_true {Γ} : ⟬Γ⟭ -> ⟬Γ,∙bool ⟭ := *)
-  (*   applyRel _ _ (mk_point (Γ R=> (Γ,∙bool)) subst_true subst_true (fun _ _ γ => ⟨γ, erefl⟩)). *)
-  (* Definition subst_false {Γ} : Γ -> Γ × bool := fun γ => ⟨γ, false⟩. *)
-  (* Definition rel_subst_false {Γ} : ⟬Γ⟭ -> ⟬Γ,∙bool ⟭ := *)
-  (*   applyRel _ _ (mk_point (Γ R=> (Γ,∙bool)) subst_false subst_false (fun _ _ γ => ⟨γ, erefl⟩)). *)
-
-  (* Definition extend_Lo {Γ A} (γ:⟬Γ⟭) (a1 a2 : A) (H : a1 = a2) : ⟬Γ,∙A⟭ := *)
-  (*   mk_point (Γ,∙A) ⟨πl γ,a1⟩ ⟨πr γ, a2⟩ ⟨πw γ, H⟩. *)
-
-  (* Lemma ValidBoolElim Γ A1 A2 m1 wm1 m2 wm2 wmrel: *)
-  (*   valid Γ A1 A2 (m1 \o subst_true) (wm1 \o subst_true) *)
-  (*         (m2 \o subst_true) (wm2 \o subst_true) (wmrel \o rel_subst_true) -> *)
-  (*   valid Γ A1 A2 (m1 \o subst_false) (wm1 \o subst_false) *)
-  (*         (m2 \o subst_false) (wm2 \o subst_false) (wmrel \o rel_subst_false) -> *)
-  (*     valid (Γ ,∙ bool) A1 A2 m1 wm1 m2 wm2 wmrel. *)
-  (* Proof. *)
-  (*   move=> [[Ht1 Ht2] Ht] [[Hf1 Hf2] Hf]; split; [split|]. *)
-  (*   move=> [γ []]; [apply Ht1| apply Hf1]. *)
-  (*   move=> [γ []]; [apply Ht2| apply Hf2]. *)
-  (*   move=> [[[γ1 []] [γ2 b2]] [γ b]] /= ; *)
-  (*   pattern b2, b; *)
-  (*   match goal with *)
-  (*   | [|- ?g _ _] => *)
-  (*     refine (match b as Hb in _ = b' return g b' Hb with | erefl => _ end) *)
-  (*   end; *)
-  (*   set γ' := mk_point _ γ1 γ2 γ. *)
-  (*   exact: (Ht γ'). *)
-  (*   exact: (Hf γ'). *)
-  (* Qed. *)
-
-  (* Definition subst_nil {Γ A} : Γ -> Γ × list A := fun γ => ⟨γ, nil⟩. *)
-
-  (* Definition rel_subst_nil {Γ A} : ⟬Γ⟭ -> ⟬Γ ,∙ list A⟭ := *)
-  (*   fun γ => mk_point (Γ ,∙ list A) (subst_nil (πl γ)) (subst_nil (πr γ)) *)
-  (*                 ⟨πw γ, eq_refl⟩. *)
-
-  (* Definition subst_cons {Γ A} : Γ × A × list A -> Γ × list A := *)
-  (*   fun γal => ⟨nfst (nfst γal), cons (nsnd (nfst γal)) (nsnd γal)⟩. *)
-
-  (* Program Definition rel_subst_cons {Γ A} : ⟬Γ,∙A,∙list A⟭ -> ⟬Γ ,∙ list A⟭ := *)
-  (*   fun γ => mk_point (Γ ,∙ list A) (subst_cons (πl γ)) (subst_cons (πr γ)) *)
-  (*                 ⟨nfst (nfst (πw γ)), eq_refl⟩. *)
-  (* Next Obligation. move: γ=> [? [[?]]] /= -> -> //. Qed. *)
-
-  (* Definition ctx_subst_extend {A Γ' Γ} (σ: Γ' R==> Γ) : (Γ' ,∙ A) R==> (Γ ,∙ A) *)
-  (*   := *)
-  (*     mk_point ((Γ' ,∙ A) R=> (Γ ,∙ A)) (fun e => ⟨(πl σ) (nfst e), nsnd e⟩) *)
-  (*              (fun e => ⟨(πr σ) (nfst e), nsnd e⟩) (fun xl xr X => ⟨(πw σ) (nfst xl) (nfst xr) (nfst X), nsnd X⟩). *)
-
-  (* Lemma ValidListElim Γ A A1 A2 m1 wm1 m2 wm2 wmrel : *)
-  (*   valid Γ A1 A2 *)
-  (*         (m1 \o subst_nil) (wm1 \o subst_nil) *)
-  (*         (m2 \o subst_nil) (wm2 \o subst_nil) *)
-  (*         (wmrel \o rel_subst_nil) -> *)
-  (*   (valid (Γ,∙ list A) A1 A2 m1 wm1 m2 wm2 wmrel -> *)
-  (*    valid (Γ,∙ A ,∙ list A) A1 A2 *)
-  (*          (m1 \o subst_cons) (wm1 \o subst_cons) *)
-  (*          (m2 \o subst_cons) (wm2 \o subst_cons) *)
-  (*          (wmrel \o rel_subst_cons)) -> *)
-  (*   valid (Γ,∙ list A) A1 A2 m1 wm1 m2 wm2 wmrel. *)
-  (* Proof. *)
-  (*   move=> [[Hnil1 Hnil2] Hnil] Hcons ; split; [split|]. *)
-
-
-  (* Definition bindStrongRSM {Γ A1 A2 B1 B2} *)
-  (*            (wm1 : πl Γ -> W1 A1) *)
-  (*            (wm2 : πr Γ -> W2 A2) *)
-  (*            (wmrel : ⟬Γ⟭ -> W A1 A2) *)
-  (*            (wf1 : πl Γ × A1 -> W1 B1) *)
-  (*            (wf2 : πr Γ × A2 -> W2 B2) *)
-  (*            (wfrel : ⟬extends Γ A1 A2⟭ -> W B1 B2) *)
-  (* : ⟬Γ⟭ -> Wrel B1 B2 *)
-
-  (* Definition to_ordProd (Γ : ) *)
-  (*            (c1 : OrdCat⦅πl Γ;M1 A1⦆) *)
-  (*            (c2 : OrdCat⦅πr Γ;M2 A2⦆) *)
-  (*            OrdCat⦅⟬Γ⟭; Jprod ⟨M1 A1, M2 A2⟩⦆ *)
-
-
-  (* Notation " Γ ⊫ c1 ≈ c2 [{ w1 , w2 , w }]" := *)
-  (*   ((θ1 _ ∙ c1 ⪷ w1) s/\ (θ2 _ ∙ c2 ⪷ w2) s/\ *)
-  (*    (orall γ : ⟬Γ⟭, θW∙1 ⟨c1 (πl γ), c2 (πr γ)⟩ ≤ w∙1 (dfst γ))) *)
-  (*     (at level 85). *)
-
 
 End RelationalProgramLogicFromRelativeMonad.
